Kraken/Examples/Move2RegsToHeapNew.lean
@@ -22,19 +22,20 @@ theorem move2_correct (env₀ : Env) (s₀ : MachineData) (a0 a8 : BitVec 64)
     (ha0 : AddrExpr.interp env₀.labels (.mk .W64) ae0 s₀.regs (.mk 0 (0 + Int64.ofNat env₀.curSize)) = a0)
     (ha8 : AddrExpr.interp env₀.labels (.mk .W64) ae8 s₀.regs (.mk 0 (0 + Int64.ofNat env₀.curSize)) = a8)
     (ha8' : AddrExpr.interp env₀.labels (.mk .W64) ae8
-        (s₀.regs.set64 .r12 (.ofBitVec (BitVec.ofInt 64 (s₀.regs.get64 .rax).toBitVec.toInt))) (.mk 0 (0 + Int64.ofNat env₀.curSize)) = a8)
+        (s₀.regs.set64 .r12 ((BitVec.ofInt 64 (s₀.regs.get64 .rax).toInt))) (.mk 0 (0 + Int64.ofNat env₀.curSize)) = a8)
     (v0 v8 : Int)
     (h_map0 : Mem.loadInt s₀.dmem a0 8 = some v0)
-    (h_map8 : Mem.loadInt (Mem.storeInt s₀.dmem a0 8 (s₀.regs.get64 .rax).toBitVec.toInt) a8 8 = some v8)
+    (h_map8 : Mem.loadInt (Mem.storeInt s₀.dmem a0 8 (s₀.regs.get64 .rax).toInt) a8 8 = some v8)
     (h_load0 : Mem.loadInt
-        (Mem.storeInt (Mem.storeInt s₀.dmem a0 8 (s₀.regs.get64 .rax).toBitVec.toInt) a8 8
-          (s₀.regs.get64 .rcx).toBitVec.toInt) a0 8 = some (s₀.regs.get64 .rax).toBitVec.toInt)
+        (Mem.storeInt (Mem.storeInt s₀.dmem a0 8 (s₀.regs.get64 .rax).toInt) a8 8
+          (s₀.regs.get64 .rcx).toInt) a0 8 = some (s₀.regs.get64 .rax).toInt)
     (h_load8 : Mem.loadInt
-        (Mem.storeInt (Mem.storeInt s₀.dmem a0 8 (s₀.regs.get64 .rax).toBitVec.toInt) a8 8
-          (s₀.regs.get64 .rcx).toBitVec.toInt) a8 8 = some (s₀.regs.get64 .rcx).toBitVec.toInt) :
+        (Mem.storeInt (Mem.storeInt s₀.dmem a0 8 (s₀.regs.get64 .rax).toInt) a8 8
+          (s₀.regs.get64 .rcx).toInt) a8 8 = some (s₀.regs.get64 .rcx).toInt) :
     ⦃fun env rip sd => env = env₀ ∧ rip = 0 ∧ sd = ⟨s₀, ()⟩⦄ move2Prog
-      ⦃fun _ _ _ s => (s.machine.regs.get64 .r12).toBitVec = (s₀.regs.get64 .rax).toBitVec ∧
-        (s.machine.regs.get64 .r13).toBitVec = (s₀.regs.get64 .rcx).toBitVec ∧
+      ⦃fun _ _ _ s => (s.machine.regs.get64 .r12) = (s₀.regs.get64 .rax) ∧
+        (s.machine.regs.get64 .r13) = (s₀.regs.get64 .rcx) ∧
         s.machine.regs.rdi = s₀.regs.rdi; fun _ _ => True⦄ := by
   vcgen [move2Prog] with (first (easm) (skip))
-  all_goals (simp_all [BitVec.ofInt_toInt] <;> bv_decide)
+  simp_all
+  -- all_goals (simp_all [BitVec.ofInt_toInt] <;> bv_decide)
